case_studies/HamiltonBlum/Blum_Completeness.ec
@@ -19,12 +19,11 @@ qed.
 
 
 local lemma hc_complete_hoare pa wa : completeness_relation pa wa =>
-   hoare[ Completeness(HonestProver, HV).run : arg = (pa,wa) ==> res ].
+   hoare[ Completeness(HP, HV).run : arg = (pa,wa) ==> res ].
 move => ishc. proc. inline*. wp. rnd. 
 wp. rnd. wp. rnd. wp. skip.
 progress.
 pose b1 := ch.
-
 case (b1 = true). 
 move => h. rewrite h. simplify.
   + have ->: (zip (unzip1 pi_gwco) (unzip2 pi_gwco)) = pi_gwco. rewrite zip_unzip. auto.
@@ -42,24 +41,26 @@ move => q.
 apply (sub_all (fun (xy : bool * (commitment * opening)) => xy.`2 \in Com xy.`1) Ver) .
 simplify. apply Com_sound.  auto.
 have f1 : size pi_gwco = size (permute_graph prm s{hr}).
-smt.
+smt(size_map permute_graph_prop2 supp_djoin_size).
 have f2 : size pi_gwco = size (unzip1 pi_gwco).
-smt.
+smt (size_map).
 rewrite - f2. 
 rewrite f1.
 rewrite permute_graph_prop2.
-split. smt. split. smt. smt.
+split. smt(). split. smt(). split. smt(size_map permute_graph_prop2 supp_djoin_size).
+smt().
 move => p.
-have ->: b1 = false. smt.
+have ->: b1 = false. smt().
 simplify. clear p. progress.
-elim ishc. smt.
-smt.  
-have : size pi_gwco = size (permute_graph prm s{hr}). smt.
-have ->: size (permute_graph prm s{hr}) = size s{hr}. smt. 
-have ->: size s{hr} = K * K. elim ishc. smt.
+elim ishc. progress. smt(size_map). smt(size_map permute_graph_prop2 supp_djoin_size).
+have : size pi_gwco = size (permute_graph prm s{hr}). smt(size_map permute_graph_prop2 supp_djoin_size lemma1).
+have ->: size (permute_graph prm s{hr}) = size s{hr}. smt (permute_graph_prop2). 
+have ->: size s{hr} = K * K. elim ishc. smt().
 move => q. 
-have qqq : size (prj_path (permute_witness prm w{hr}) pi_gwco) = K.
-smt. smt.
+have qqq : size (prj_path (permute_witness prm w{hr}) pi_gwco) = K.   
+rewrite lemma1.  rewrite q. rewrite size_map. elim ishc. smt().
+elim ishc. smt(size_map).
+smt (size_map).
 have ->: (prj_path (permute_witness prm w{hr}) (unzip1 pi_gwco))
   = (unzip1 (prj_path (permute_witness prm w{hr}) pi_gwco)).
 rewrite lemma2. auto.
@@ -78,9 +79,10 @@ apply Com_sound.
 have : x1.`1 \in (nseq K true). 
  have md : (prj_path (permute_witness prm w{hr}) (permute_graph prm s{hr}))
    = (prj_path (w{hr}) (s{hr})).
-smt (prj_lemma). smt.
+smt (prj_lemma). 
+smt (mem_zip_fst).
 have : x1.`2 \in (prj_path (permute_witness prm w{hr}) pi_gwco).
-   smt.
+   smt(mem_zip_snd).
  move => qq.
 have : x1.`2 \in pi_gwco. apply (lemma5 x1.`2 (permute_witness prm w{hr})). auto.
 move => qqq.
@@ -95,52 +97,53 @@ have H6' :
 rewrite - lemma8. auto.
 rewrite  (lemma5 x1 (permute_witness prm w{hr})). apply H6'.
 smt(lemma7 perm_eq_trans).
-smt.
+smt().
 qed.
 
 
 local lemma hc_complete statement witness &m : completeness_relation statement witness =>
-  Pr[Completeness(HonestProver, HV).run(statement, witness) @ &m : true] = 1%r.
-move => inlang. byphoare (_: arg = (statement, witness) ==> _);auto. proc. inline*. wp. rnd.  simplify. wp. 
+  Pr[Completeness(HP, HV).run(statement, witness) @ &m : true] = 1%r.
+move => inlang. byphoare (_: arg = (statement, witness) ==> _);auto. 
+proc. inline*. wp. rnd.  simplify. wp. 
 rnd.  wp. 
 conseq (_: _ ==> true). progress. smt (@Distr @DBool). 
 apply djoinmap_weight. apply Com_lossless.
-rnd. wp.  skip. progress. apply perm_d_lossless. (* smt (ishc_prop2).  *)
+rnd. wp.  skip. progress. apply perm_d_lossless.
 qed.
 
 
 local lemma hc_complete_failure statement witness &m : 
  completeness_relation statement witness =>
-   Pr[Completeness(HonestProver, HV).run(statement, witness) @ &m : !res] = 0%r.
+   Pr[Completeness(HP, HV).run(statement, witness) @ &m : !res] = 0%r.
 progress. byphoare (_: arg = (statement,witness) ==> _);auto.
 hoare. simplify. conseq (hc_complete_hoare statement witness H).
 qed.
 
 
-lemma hc_completeness: forall (statement : hc_prob) (witness : hc_wit) &m,
+lemma hc_completeness: forall (statement : hc_stat) (witness : hc_wit) &m,
         completeness_relation statement witness =>
-     Pr[Completeness(HonestProver, HV).run(statement, witness) 
+     Pr[Completeness(HP, HV).run(statement, witness) 
             @ &m : res] = 1%r.
 progress. 
 rewrite - (hc_complete statement witness &m H).
 have f : 0%r = 
- Pr[Completeness(HonestProver, HV).run(statement, witness) @ &m : true]
-  - Pr[Completeness(HonestProver, HV).run(statement, witness) @ &m : res].
+ Pr[Completeness(HP, HV).run(statement, witness) @ &m : true]
+  - Pr[Completeness(HP, HV).run(statement, witness) @ &m : res].
 rewrite Pr[mu_split res].  
 rewrite hc_complete_failure;auto. 
-smt.
+smt().
 qed.
 
 
 (* iterated completeness for Blum protocol  *)
-lemma hc_completeness_iter: forall (statement:hc_prob) (witness:hc_wit) &m n,
+lemma hc_completeness_iter: forall (statement:hc_stat) (witness:hc_wit) &m n,
         1 <= n =>
        completeness_relation statement witness =>
-      Pr[CompletenessAmp(HonestProver,HV).run(statement, witness,n) @ &m : res] = 1%r.
+      Pr[CompletenessAmp(HP,HV).run(statement, witness,n) @ &m : res] = 1%r.
 progress.
-apply (BlumProtocol.CompletenessTheory.Perfect.completeness_seq HonestProver HV _ _ _ _ _ &m).
+apply (BlumProtocol.CompletenessTheory.Perfect.completeness_seq HP HV _ _ _ _ _ &m).
 proc.  skip.  auto.
-proc.  wp.  rnd.  skip.  progress. smt.
+proc.  wp.  rnd.  skip.  progress. smt (@Distr).
 proc.  wp.  skip. auto.
 proc. rnd. conseq (_: _ ==> true). progress. smt(djoinmap_weight Com_lossless). wp. rnd. wp. skip. smt (perm_d_lossless).
 progress.
